src/ocaml-output/FStar_Tactics_Basic.ml
@@ -11,36 +11,42 @@ let (core_check :
     fun sol ->
       fun t ->
         fun must_tot ->
-          let debug f =
-            let uu___ = FStar_Options.debug_any () in
-            if uu___ then f () else () in
-          let uu___ = FStar_TypeChecker_Core.check_term env sol t must_tot in
-          match uu___ with
-          | FStar_Pervasives.Inl (FStar_Pervasives_Native.None) ->
-              (debug
-                 (fun uu___2 ->
-                    FStar_Compiler_Util.print_string
-                      "Core check ok (no guard)\n");
-               FStar_Pervasives.Inl FStar_Pervasives_Native.None)
-          | FStar_Pervasives.Inl (FStar_Pervasives_Native.Some g) ->
-              (debug
-                 (fun uu___2 ->
-                    FStar_Compiler_Util.print_string "Core check ok\n");
-               FStar_Pervasives.Inl (FStar_Pervasives_Native.Some g))
-          | FStar_Pervasives.Inr err ->
-              (debug
-                 (fun uu___2 ->
-                    let uu___3 =
-                      let uu___4 = FStar_TypeChecker_Env.get_range env in
-                      FStar_Compiler_Range.string_of_range uu___4 in
-                    let uu___4 = FStar_TypeChecker_Core.print_error_short err in
-                    let uu___5 = FStar_Syntax_Print.term_to_string sol in
-                    let uu___6 = FStar_Syntax_Print.term_to_string t in
-                    let uu___7 = FStar_TypeChecker_Core.print_error err in
-                    FStar_Compiler_Util.print5
-                      "(%s) Core checking failed (%s) on term %s and type %s\n%s\n"
-                      uu___3 uu___4 uu___5 uu___6 uu___7);
-               FStar_Pervasives.Inr err)
+          let uu___ = FStar_Options.admit_tactic_unification_guards () in
+          if uu___
+          then FStar_Pervasives.Inl FStar_Pervasives_Native.None
+          else
+            (let debug f =
+               let uu___2 = FStar_Options.debug_any () in
+               if uu___2 then f () else () in
+             let uu___2 =
+               FStar_TypeChecker_Core.check_term env sol t must_tot in
+             match uu___2 with
+             | FStar_Pervasives.Inl (FStar_Pervasives_Native.None) ->
+                 (debug
+                    (fun uu___4 ->
+                       FStar_Compiler_Util.print_string
+                         "Core check ok (no guard)\n");
+                  FStar_Pervasives.Inl FStar_Pervasives_Native.None)
+             | FStar_Pervasives.Inl (FStar_Pervasives_Native.Some g) ->
+                 (debug
+                    (fun uu___4 ->
+                       FStar_Compiler_Util.print_string "Core check ok\n");
+                  FStar_Pervasives.Inl (FStar_Pervasives_Native.Some g))
+             | FStar_Pervasives.Inr err ->
+                 (debug
+                    (fun uu___4 ->
+                       let uu___5 =
+                         let uu___6 = FStar_TypeChecker_Env.get_range env in
+                         FStar_Compiler_Range.string_of_range uu___6 in
+                       let uu___6 =
+                         FStar_TypeChecker_Core.print_error_short err in
+                       let uu___7 = FStar_Syntax_Print.term_to_string sol in
+                       let uu___8 = FStar_Syntax_Print.term_to_string t in
+                       let uu___9 = FStar_TypeChecker_Core.print_error err in
+                       FStar_Compiler_Util.print5
+                         "(%s) Core checking failed (%s) on term %s and type %s\n%s\n"
+                         uu___5 uu___6 uu___7 uu___8 uu___9);
+                  FStar_Pervasives.Inr err))
 type name = FStar_Syntax_Syntax.bv
 type env = FStar_TypeChecker_Env.env
 type implicits = FStar_TypeChecker_Env.implicits
