src/syntax/FStar.Syntax.Hash.fst
@@ -23,75 +23,135 @@ open FStar.Const
 module SS = FStar.Syntax.Subst
 module UU = FStar.Syntax.Unionfind
 
+(* maybe memo *)
+let mm (t:Type) = bool -> t & bool
+
+let (let?) (f:mm 't) (g: 't -> mm 's) : mm 's = 
+  fun b -> 
+    let t, b = f b in
+    g t b
+
+let ret (x:'t) : mm 't = fun b -> x, b
+
+let should_memo : mm bool = fun b -> b, b
+
+let no_memo : mm unit = fun _ -> (), false
+
 module H = FStar.Hash
-inline_for_extraction
-let memoize (h:syntax 'a) (f:syntax 'a -> H.hash_code) : H.hash_code =
-  match !h.hash_code with
-  | Some c -> c
-  | None ->
-    let c = f h in
-    h.hash_code := Some c;
-    c
-let rec mix_list (l:list H.hash_code) : H.hash_code =
-  match l with
-  | [] -> H.of_int 1229
-  | hd::tl -> H.mix (H.of_int 1231) (H.mix hd (mix_list tl))
-let hash_list (h:'a -> H.hash_code) (ts:list 'a) : H.hash_code = mix_list (List.map h ts)
-let hash_array (h:'a -> H.hash_code) (ts:array 'a) : H.hash_code = admit()
-let hash_option (h:'a -> H.hash_code) (o:option 'a) : H.hash_code =
+
+let maybe_memoize (h:syntax 'a) (f:syntax 'a -> mm H.hash_code) : mm H.hash_code =
+  fun should_memo ->
+    if should_memo 
+    then (
+      match !h.hash_code with
+      | Some c -> c, should_memo
+      | None ->
+        let c, should_memo = f h should_memo in
+        if should_memo 
+        then h.hash_code := Some c;
+        c, should_memo
+    )
+    else f h should_memo
+
+let of_int (i:int) : mm H.hash_code = ret (H.of_int i)
+
+let of_string (s:string) : mm H.hash_code = ret (H.of_string s)
+
+let mix (f:mm H.hash_code) (g:mm H.hash_code) : mm H.hash_code =
+  fun b -> let x, b0 = f b in
+        let y, b1 = g b in
+        H.mix x y, b0 && b1
+
+let nil_hc : mm H.hash_code = of_int 1229
+let cons_hc : mm H.hash_code = of_int 1231
+
+let mix_list (l:list (mm H.hash_code)) : mm H.hash_code = 
+  List.fold_right (fun i out -> mix cons_hc (mix i out)) l nil_hc
+
+let mix_list_lit = mix_list
+
+let hash_list (h:'a -> mm H.hash_code) (ts:list 'a) : mm H.hash_code = mix_list (List.map h ts)
+
+let hash_array (h:'a -> mm H.hash_code) (ts:array 'a) : mm H.hash_code = admit()
+
+let hash_option (h:'a -> mm H.hash_code) (o:option 'a) : mm H.hash_code =
   match o with
-  | None -> H.of_int 1237
-  | Some o -> H.mix (H.of_int 1249) (h o)
-inline_for_extraction
-let hash_pair (h:'a -> H.hash_code) (i:'b -> H.hash_code) (x:('a * 'b)) =
-  H.mix (h (fst x)) (i (snd x))
-inline_for_extraction
-let hash_list_lit (h:'a -> H.hash_code) (ts:list 'a) : H.hash_code =
-  Pervasives.norm [zeta_full; delta_only [`%hash_list; `%List.map]; iota] (hash_list h ts)
-let mix_list_lit (l:list H.hash_code) : H.hash_code =
-  Pervasives.norm [zeta_full; delta_only [`%mix_list]; iota] (mix_list l)
-let hash_byte (b:FStar.BaseTypes.byte) : H.hash_code = H.of_int (UInt8.v b)
-let rec hash_term (t:term)
-  : H.hash_code
-  = memoize t hash_term'
+  | None -> ret (H.of_int 1237)
+  | Some o -> mix (ret (H.of_int 1249)) (h o)
+
+
+let hash_pair (h:'a -> mm H.hash_code) (i:'b -> mm H.hash_code) (x:('a * 'b))
+  : mm H.hash_code
+  = mix (h (fst x)) (i (snd x))
+
+let hash_byte (b:FStar.BaseTypes.byte) : mm H.hash_code = ret (H.of_int (UInt8.v b))
+
+let rec hash_term (t:term) 
+  : mm H.hash_code
+  = maybe_memoize t hash_term'
+
+and hash_comp c
+  : mm H.hash_code
+  = maybe_memoize c hash_comp'
 
 and hash_term' (t:term)
-  : H.hash_code
-  //Primes: 1 -- 40
+  : mm H.hash_code
   = match (SS.compress t).n with
-    | Tm_bvar bv -> H.mix (H.of_int 3) (H.of_int bv.index)
-    | Tm_name bv -> H.mix (H.of_int 5) (H.of_int bv.index)
-    | Tm_fvar fv -> H.mix (H.of_int 7) (hash_fv fv)
-    | Tm_uinst(t, us) -> H.mix (H.of_int 11)
-                                   (H.mix (hash_term t)
+    | Tm_bvar bv -> mix (of_int 3) (of_int bv.index)
+    | Tm_name bv -> mix (of_int 5) (of_int bv.index)
+    | Tm_fvar fv -> mix (of_int 7) (hash_fv fv)
+    | Tm_uinst(t, us) -> mix (of_int 11)
+                                   (mix (hash_term t)
                                                (hash_list hash_universe us))
-    | Tm_constant sc -> H.mix (H.of_int 13) (hash_constant sc)
-    | Tm_type u -> H.mix (H.of_int 17) (hash_universe u)
-    | Tm_abs(bs, t, rcopt) -> H.mix (H.of_int 19)
-                                        (H.mix (hash_list hash_binder bs)
-                                                    (H.mix (hash_term t)
+    | Tm_constant sc -> mix (of_int 13) (hash_constant sc)
+    | Tm_type u -> mix (of_int 17) (hash_universe u)
+    | Tm_abs(bs, t, rcopt) -> mix (of_int 19)
+                                        (mix (hash_list hash_binder bs)
+                                                    (mix (hash_term t)
                                                                 (hash_option hash_rc rcopt)))
-    | Tm_arrow(bs, c) -> H.mix (H.of_int 23) (hash_comp c)
-    | Tm_refine(b, t) -> H.mix (H.of_int 29) (H.mix (hash_bv b) (hash_term t))
-    | Tm_app (t, args) -> H.mix (H.of_int 31) (H.mix (hash_term t) (hash_list hash_arg args))
+    | Tm_arrow(bs, c) -> mix (of_int 23) (mix (hash_list hash_binder bs) (hash_comp c))
+    | Tm_refine(b, t) -> mix (of_int 29) (mix (hash_bv b) (hash_term t))
+    | Tm_app (t, args) -> mix (of_int 31) (mix (hash_term t) (hash_list hash_arg args))
     | Tm_match (t, asc_opt, branches, rcopt) ->
-      H.mix (H.of_int 37) 
-            (H.mix (hash_option hash_match_returns asc_opt)
-                   (H.mix (H.mix (hash_term t) (hash_list hash_branch branches))
+      mix (of_int 37) 
+            (mix (hash_option hash_match_returns asc_opt)
+                   (mix (mix (hash_term t) (hash_list hash_branch branches))
                           (hash_option hash_rc rcopt)))
-    | Tm_ascribed(t, a, lopt) -> H.mix (H.of_int 43) (H.mix (hash_term t) (H.mix (hash_ascription a) (hash_option hash_lid lopt)))
-    | Tm_let((false, [lb]), t) -> H.mix (H.of_int 47) (H.mix (hash_lb lb) (hash_term t))
-    | Tm_let((_, lbs), t) -> H.mix (H.of_int 51) (H.mix (hash_list hash_lb lbs) (hash_term t))
-    | Tm_uvar uv -> H.mix (H.of_int 53) (hash_uvar uv)
-    | Tm_meta(t, m) -> H.mix (H.of_int 61) (hash_meta m)
-    | Tm_lazy li -> H.mix (H.of_int 67) (hash_lazyinfo li)
-    | Tm_quoted (t, qi) -> H.mix (H.of_int 71) (hash_quoteinfo qi)
-    | Tm_unknown -> H.of_int 73
+    | Tm_ascribed(t, a, lopt) -> mix (of_int 43) (mix (hash_term t) (mix (hash_ascription a) (hash_option hash_lid lopt)))
+    | Tm_let((false, [lb]), t) -> mix (of_int 47) (mix (hash_lb lb) (hash_term t))
+    | Tm_let((_, lbs), t) -> mix (of_int 51) (mix (hash_list hash_lb lbs) (hash_term t))
+    | Tm_uvar uv -> mix (of_int 53) (hash_uvar uv)
+    | Tm_meta(t, m) -> mix (of_int 61) (mix (hash_term t) (hash_meta m))
+    | Tm_lazy li -> mix (of_int 67) (hash_lazyinfo li)
+    | Tm_quoted (t, qi) -> mix (of_int 71) (mix (hash_term t) (hash_quoteinfo qi))
+    | Tm_unknown -> of_int 73
     | Tm_delayed _ -> failwith "Impossible"
+
+and hash_comp' (c:comp)
+  : mm H.hash_code
+  = match c.n with
+    | Total (t, ou) ->
+      mix_list_lit
+        [of_int 811;
+         hash_term t;
+         hash_option hash_universe ou]
+    | GTotal (t, ou) ->
+      mix_list_lit
+        [of_int 821;
+         hash_term t;
+         hash_option hash_universe ou]
+    | Comp ct ->
+      mix_list_lit
+        [of_int 823;
+         hash_list hash_universe ct.comp_univs;
+         hash_lid ct.effect_name;
+         hash_term ct.result_typ;
+         hash_list hash_arg ct.effect_args;
+         hash_list hash_flag ct.flags]
 
 and hash_lb lb =
   mix_list_lit
-    [ H.of_int 79;
+    [ of_int 79;
       hash_lbname lb.lbname;
       hash_list hash_ident lb.lbunivs;
       hash_term lb.lbtyp;
@@ -100,54 +160,33 @@ and hash_lb lb =
       hash_list hash_term lb.lbattrs]
 
 and hash_match_returns (b, asc) = 
-  H.mix (hash_binder b)
-        (hash_ascription asc)
+  mix (hash_binder b)
+      (hash_ascription asc)
         
 and hash_branch b =
   let p, topt, t = b in
   mix_list_lit
-    [H.of_int 83;
+    [of_int 83;
      hash_pat p;
      hash_option hash_term topt;
      hash_term t]
 
 and hash_pat p =
   match p.v with
-  | Pat_constant c -> H.mix (H.of_int 89) (hash_constant c)
-  | Pat_cons(fv, _us, args) ->
+  | Pat_constant c -> mix (of_int 89) (hash_constant c)
+  | Pat_cons(fv, us, args) ->
     mix_list_lit
-      [H.of_int 97;
+      [of_int 97;
        hash_fv fv;
+       hash_option (hash_list hash_universe) us;
        hash_list (hash_pair hash_pat hash_bool) args]
-  | Pat_var bv -> H.mix (H.of_int 101) (hash_bv bv)
-  | Pat_wild bv -> H.mix (H.of_int 103) (hash_bv bv)
-  | Pat_dot_term t -> mix_list_lit [H.of_int 107; hash_option hash_term t]
+  | Pat_var bv -> mix (of_int 101) (hash_bv bv)
+  | Pat_wild bv -> mix (of_int 103) (hash_bv bv)
+  | Pat_dot_term t -> mix_list_lit [of_int 107; hash_option hash_term t]
 
-and hash_comp c =
-  //Primes: 141--160
-  memoize c (fun c ->
-    match c.n with
-    | Total (t, ou) ->
-      mix_list_lit
-        [H.of_int 811;
-         hash_term t;
-         hash_option hash_universe ou]
-    | GTotal (t, ou) ->
-      mix_list_lit
-        [H.of_int 821;
-         hash_term t;
-         hash_option hash_universe ou]
-    | Comp ct ->
-      mix_list_lit
-        [H.of_int 823;
-         hash_list hash_universe ct.comp_univs;
-         hash_lid ct.effect_name;
-         hash_term ct.result_typ;
-         hash_list hash_arg ct.effect_args;
-         hash_list hash_flag ct.flags])
 
-and hash_bv b = H.mix (hash_ident b.ppname) (hash_term b.sort)
-and hash_fv fv = H.of_string (Ident.string_of_lid fv.fv_name.v)
+and hash_bv b = hash_term b.sort
+and hash_fv fv = of_string (Ident.string_of_lid fv.fv_name.v)
 and hash_binder (b:binder) =
   mix_list_lit
     [hash_bv b.binder_bv;
@@ -155,80 +194,76 @@ and hash_binder (b:binder) =
      hash_list hash_term b.binder_attrs]
 
 and hash_universe =
-  //Primes: 41 -- 60
   function
-  | U_zero -> H.of_int 179
-  | U_succ u -> H.mix (H.of_int 181) (hash_universe u)
-  | U_max us -> H.mix (H.of_int 191) (hash_list hash_universe us)
-  | U_bvar i -> H.mix (H.of_int 193) (H.of_int i)
-  | U_name i -> H.mix (H.of_int 197) (hash_ident i)
-  | U_unif uv -> H.mix (H.of_int 199) (hash_universe_uvar uv)
-  | U_unknown -> H.of_int 211
+  | U_zero -> of_int 179
+  | U_succ u -> mix (of_int 181) (hash_universe u)
+  | U_max us -> mix (of_int 191) (hash_list hash_universe us)
+  | U_bvar i -> mix (of_int 193) (of_int i)
+  | U_name i -> mix (of_int 197) (hash_ident i)
+  | U_unif uv -> mix (of_int 199) (hash_universe_uvar uv)
+  | U_unknown -> of_int 211
 
 and hash_arg (t, aq) =
-  H.mix (hash_term t) (hash_option hash_arg_qualifier aq)
+  mix (hash_term t) (hash_option hash_arg_qualifier aq)
 
 and hash_arg_qualifier aq = 
-  H.mix (hash_bool aq.aqual_implicit)
+  mix (hash_bool aq.aqual_implicit)
         (hash_list hash_term aq.aqual_attributes)
   
 and hash_bqual =
-  //Primes: 81--100
   function
-  | Implicit true -> H.of_int 419
-  | Implicit false -> H.of_int 421
-  | Meta t -> H.mix (H.of_int 431) (hash_term t)
-  | Equality -> H.of_int 433
+  | Implicit true -> of_int 419
+  | Implicit false -> of_int 421
+  | Meta t -> mix (of_int 431) (hash_term t)
+  | Equality -> of_int 433
 
-and hash_uvar (u, _) = H.of_int (UU.uvar_id u.ctx_uvar_head)
+and hash_uvar (u, _) = of_int (UU.uvar_id u.ctx_uvar_head)
 
-and hash_universe_uvar u = H.of_int (UU.univ_uvar_id u)
+and hash_universe_uvar u = of_int (UU.univ_uvar_id u)
 
 and hash_ascription (a, to, b) =
-  H.mix
+  mix
     (match a with
     | Inl t -> hash_term t
     | Inr c -> hash_comp c)
     (hash_option hash_term to)
 
 and hash_bool b =
-  if b then H.of_int 307
-  else H.of_int 311
+  if b then of_int 307
+  else of_int 311
 
 and hash_constant =
-  //Primes: 61--80
   function
-  | Const_effect -> H.of_int 283
-  | Const_unit -> H.of_int 293
+  | Const_effect -> of_int 283
+  | Const_unit -> of_int 293
   | Const_bool b -> hash_bool b
-  | Const_int (s, o) -> H.mix (H.of_int 313)
-                             (H.mix (H.of_string s)
+  | Const_int (s, o) -> mix (of_int 313)
+                             (mix (of_string s)
                                     (hash_option hash_sw o))
-  | Const_char c -> H.mix (H.of_int 317) (H.of_int (UInt32.v (Char.u32_of_char c)))
-  | Const_float d -> H.mix (H.of_int 331) (H.of_int 0) //(hash_double d)(* ?? *)
-  | Const_real s -> H.mix (H.of_int 337) (H.of_string s)
-  | Const_bytearray (bs, _) -> H.mix (H.of_int 347) (hash_array hash_byte bs)
-  | Const_string (s, _) -> H.mix (H.of_int 349) (H.of_string s)
-  | Const_range_of -> H.of_int 353
-  | Const_set_range_of -> H.of_int 359
-  | Const_range r -> H.mix (H.of_int 367) (H.of_string (Range.string_of_range r))
-  | Const_reify -> H.of_int 367
-  | Const_reflect l -> H.mix (H.of_int 373) (hash_lid l)
+  | Const_char c -> mix (of_int 317) (of_int (UInt32.v (Char.u32_of_char c)))
+  | Const_float d -> mix (of_int 331) (of_int 0) //(hash_double d)(* ?? *)
+  | Const_real s -> mix (of_int 337) (of_string s)
+  | Const_bytearray (bs, _) -> mix (of_int 347) (hash_array hash_byte bs)
+  | Const_string (s, _) -> mix (of_int 349) (of_string s)
+  | Const_range_of -> of_int 353
+  | Const_set_range_of -> of_int 359
+  | Const_range r -> mix (of_int 367) (of_string (Range.string_of_range r))
+  | Const_reify -> of_int 367
+  | Const_reflect l -> mix (of_int 373) (hash_lid l)
 
 and hash_sw (s, w) =
-  //Primes: 101-120
-  H.mix
+  mix
   (match s with
-   | Unsigned -> H.of_int 547
-   | Signed -> H.of_int 557)
+   | Unsigned -> of_int 547
+   | Signed -> of_int 557)
   (match w with
-   | Int8 -> H.of_int 563
-   | Int16 -> H.of_int 569
-   | Int32 -> H.of_int 571
-   | Int64 -> H.of_int 577)
+   | Int8 -> of_int 563
+   | Int16 -> of_int 569
+   | Int32 -> of_int 571
+   | Int64 -> of_int 577)
 
-and hash_ident i = H.of_string (Ident.string_of_id i)
-and hash_lid l = H.of_string (Ident.string_of_lid l)
+and hash_ident i = of_string (Ident.string_of_id i)
+and hash_lid l = of_string (Ident.string_of_lid l)
 and hash_lbname l =
   match l with
   | Inl bv -> hash_bv bv
@@ -239,75 +274,64 @@ and hash_rc rc =
       hash_option hash_term rc.residual_typ;
       hash_list hash_flag rc.residual_flags ]
 
-and hash_subst (s:subst_ts) : H.hash_code =
-  hash_list (hash_list hash_subst_elt) (fst s)
-
-and hash_subst_elt =
-  function
-   | DB (i, bv) -> mix_list_lit [H.of_int 1087; H.of_int i; hash_bv bv]
-   | NM (bv, i) -> mix_list_lit [H.of_int 1091; hash_bv bv; H.of_int i]
-   | NT (bv, t) -> mix_list_lit [H.of_int 1093; hash_bv bv; hash_term t]
-   | UN (i, u) -> mix_list_lit [H.of_int 1097; H.of_int i; hash_universe u]
-   | UD (un, i) -> mix_list_lit [H.of_int 1103; hash_ident un; H.of_int i]
-
 and hash_flag =
   function
-  | TOTAL -> H.of_int 947
-  | MLEFFECT -> H.of_int 953
-  | LEMMA -> H.of_int 967
-  | RETURN -> H.of_int 971
-  | PARTIAL_RETURN -> H.of_int 977
-  | SOMETRIVIAL -> H.of_int 983
-  | TRIVIAL_POSTCONDITION -> H.of_int 991
-  | SHOULD_NOT_INLINE -> H.of_int 997
-  | CPS -> H.of_int 1009
-  | DECREASES (Decreases_lex ts) -> H.mix (H.of_int 1013) (hash_list hash_term ts)
-  | DECREASES (Decreases_wf (t0, t1)) -> H.mix (H.of_int 2341) (hash_list hash_term [t0;t1])
+  | TOTAL -> of_int 947
+  | MLEFFECT -> of_int 953
+  | LEMMA -> of_int 967
+  | RETURN -> of_int 971
+  | PARTIAL_RETURN -> of_int 977
+  | SOMETRIVIAL -> of_int 983
+  | TRIVIAL_POSTCONDITION -> of_int 991
+  | SHOULD_NOT_INLINE -> of_int 997
+  | CPS -> of_int 1009
+  | DECREASES (Decreases_lex ts) -> mix (of_int 1013) (hash_list hash_term ts)
+  | DECREASES (Decreases_wf (t0, t1)) -> mix (of_int 2341) (hash_list hash_term [t0;t1])
 
 and hash_meta m =
   match m with
   | Meta_pattern (ts, args) ->
     mix_list_lit
-      [ H.of_int 1019;
+      [ of_int 1019;
         hash_list hash_term ts;
         hash_list (hash_list hash_arg) args ]
   | Meta_named l ->
     mix_list_lit
-      [ H.of_int 1021;
+      [ of_int 1021;
         hash_lid l ]
   | Meta_labeled (s, r, _) ->
     mix_list_lit
-      [ H.of_int 1031;
-        H.of_string s;
-        H.of_string (Range.string_of_range r) ]
+      [ of_int 1031;
+        of_string s;
+        of_string (Range.string_of_range r) ]
   | Meta_desugared msi ->
     mix_list_lit
-      [ H.of_int 1033;
+      [ of_int 1033;
         hash_meta_source_info msi ]
   | Meta_monadic(m, t) ->
     mix_list_lit
-      [ H.of_int 1039;
+      [ of_int 1039;
         hash_lid m;
         hash_term t ]
   | Meta_monadic_lift (m0, m1, t) ->
     mix_list_lit
-      [H.of_int 1069;
+      [of_int 1069;
        hash_lid m0;
        hash_lid m1;
        hash_term t]
 
 and hash_meta_source_info m =
    match m with
-   | Sequence -> H.of_int 1049
-   | Primop -> H.of_int 1051
-   | Masked_effect -> H.of_int 1061
-   | Meta_smt_pat -> H.of_int 1063
-   | Machine_integer sw -> H.mix (H.of_int 1069) (hash_sw sw)
+   | Sequence -> of_int 1049
+   | Primop -> of_int 1051
+   | Masked_effect -> of_int 1061
+   | Meta_smt_pat -> of_int 1063
+   | Machine_integer sw -> mix (of_int 1069) (hash_sw sw)
 
-and hash_lazyinfo li = H.of_int 0 //no meaningful way to hash the blob
+and hash_lazyinfo li = of_int 0 //no meaningful way to hash the blob
 
 and hash_quoteinfo qi =
-  H.mix
+  mix
     (hash_bool (qi.qkind = Quote_static))
     (hash_list (hash_pair hash_bv hash_term) qi.antiquotes)
 
@@ -328,10 +352,13 @@ let equal_pair f g (x1, y1) (x2, y2) = f x1 x2 && g y1 y2
 
 let equal_poly x y = x=y
 
+let ext_hash_term (t:term) = fst (hash_term t true)
+let ext_hash_term_no_memo (t:term) = fst (hash_term t false)
+
 let rec equal_term (t1 t2:term)
   : bool
   = if physical_equality t1 t2 then true else
-    if hash_term t1 <> hash_term t2 then false else
+    if ext_hash_term t1 <> ext_hash_term t2 then false else
     match (SS.compress t1).n, (SS.compress t2).n with
     | Tm_bvar x, Tm_bvar y -> x.index = y.index
     | Tm_name x, Tm_name y -> x.index = y.index
@@ -578,3 +605,4 @@ and equal_subst_elt s1 s2 =
   | UD (un1, i1), UD (un2, i2) ->
     i1 = i2 &&
     Ident.ident_equals un1 un2
+
