src/tactics/FStar.Tactics.Monad.fst
@@ -47,6 +47,7 @@ let incr_goal_ctr () = let v = !goal_ctr in goal_ctr := v + 1; v
 
 let register_goal (env:Env.env) (uv:S.ctx_uvar) =
       let i = Core.incr_goal_ctr () in
+      // if Options.admit_tactic_unification_guards() then () else
       let env = {env with gamma = uv.ctx_uvar_gamma } in
       if Env.debug env <| Options.Other "Core"
       ||  Env.debug env <| Options.Other "RegisterGoal"
