src/typechecker/FStar.TypeChecker.Core.fst
@@ -205,7 +205,11 @@ type hash_entry = {
 }
 
 type tc_table = FStar.Hash.hashtable term hash_entry
-let table : tc_table = FStar.Hash.create FStar.Syntax.Hash.equal_term
+let equal_term_for_hash t1 t2 = 
+  Profiling.profile (fun _ -> Hash.equal_term t1 t2) None "FStar.TypeChecker.Core.equal_term_for_hash"
+let equal_term t1 t2 =  
+  Profiling.profile (fun _ -> Hash.equal_term t1 t2) None "FStar.TypeChecker.Core.equal_term"
+let table : tc_table = FStar.Hash.create equal_term_for_hash
 type cache_stats_t = { hits : int; misses : int }
 let cache_stats = Util.mk_ref { hits = 0; misses = 0 }
 let record_cache_hit () =
@@ -225,7 +229,7 @@ let insert (g:env) (e:term) (res:success (effect_label & typ)) =
        he_res = res
     }
     in
-    FStar.Hash.insert (e, FStar.Syntax.Hash.hash_term) entry table
+    FStar.Hash.insert (e, FStar.Syntax.Hash.ext_hash_term) entry table
 
 inline_for_extraction
 let return (#a:Type) (x:a) : result a = fun _ -> Inl (x, None)
@@ -524,7 +528,7 @@ let rec context_included (g0 g1: list binding) =
      match b0, b1 with
      | Binding_var x0, Binding_var x1 ->
        if x0.index = x1.index
-       then Hash.equal_term x0.sort x1.sort
+       then equal_term x0.sort x1.sort
             && context_included g0' g1'
        else context_included g0 g1'
 
@@ -545,7 +549,7 @@ let curry_application hd arg args p =
 
 
 let lookup (g:env) (e:term) : result (effect_label & typ) =
-   match FStar.Hash.lookup (e, FStar.Syntax.Hash.hash_term) table with
+   match FStar.Hash.lookup (e, FStar.Syntax.Hash.ext_hash_term) table with
    | None -> fail "not in cache"
    | Some he ->
      if he.he_gamma `context_included` g.tcenv.gamma
@@ -681,7 +685,7 @@ let rec check_relation (g:env) (rel:relation) (t0 t1:typ)
         match (U.un_uinst head0).n, (U.un_uinst head1).n with
         | Tm_fvar fv0, Tm_fvar fv1 -> fv_eq fv0 fv1
         | Tm_name x0, Tm_name x1 -> bv_eq x0 x1
-        | Tm_constant c0, Tm_constant c1 -> Hash.equal_term head0 head1
+        | Tm_constant c0, Tm_constant c1 -> equal_term head0 head1
         | Tm_type _, Tm_type _ 
         | Tm_arrow _, Tm_arrow _
         | Tm_match _, Tm_match _ -> true
@@ -711,7 +715,8 @@ let rec check_relation (g:env) (rel:relation) (t0 t1:typ)
     in
     let maybe_unfold_side side t0 t1
       : option (term & term)
-      = match side with
+      = Profiling.profile (fun _ -> 
+        match side with
         | Neither -> None
         | Both -> (
           match N.maybe_unfold_head g.tcenv t0, 
@@ -731,7 +736,9 @@ let rec check_relation (g:env) (rel:relation) (t0 t1:typ)
           match N.maybe_unfold_head g.tcenv t1 with
           | Some t1 -> Some (t0, t1)
           | _ -> None
-        )
+        ))
+        None
+        "FStar.TypeChecker.Core.maybe_unfold_side"
     in
     let maybe_unfold t0 t1
       : option (term & term)
@@ -773,13 +780,19 @@ let rec check_relation (g:env) (rel:relation) (t0 t1:typ)
           
         | _ -> t
     in
+    let beta_iota_reduce t =
+        Profiling.profile
+          (fun () -> beta_iota_reduce t)
+          None
+          "FStar.TypeChecker.Core.beta_iota_reduce"
+    in
     let t0 = Subst.compress (beta_iota_reduce t0) in
     let t1 = Subst.compress (beta_iota_reduce t1) in
     let check_relation g rel t0 t1 =
       with_context "check_relation" (Some (CtxRel t0 rel t1)) 
         (fun _ -> check_relation g rel t0 t1)
     in
-    if Hash.equal_term t0 t1 then return ()
+    if equal_term t0 t1 then return ()
     else 
       match t0.n, t1.n with
       | Tm_type u0, Tm_type u1 ->
@@ -804,7 +817,7 @@ let rec check_relation (g:env) (rel:relation) (t0 t1:typ)
         check_relation g rel t0 t1
 
       | Tm_uinst (f0, us0), Tm_uinst(f1, us1) ->
-        if Hash.equal_term f0 f1
+        if equal_term f0 f1
         then ( //heads are equal, equate universes
              if Rel.teq_nosmt_force g.tcenv t0 t1
              then return ()
@@ -1045,8 +1058,15 @@ and check_relation_comp (g:env) rel (c0 c1:comp)
 
 
 and check_subtype (g:env) (e:option term) (t0 t1:typ)
-  = let rel = SUBTYPING e in
-    with_context "check_subtype" (Some (CtxRel t0 rel t1)) (fun _ -> check_relation g rel t0 t1)
+  = fun ctx ->
+    Profiling.profile
+      (fun () -> 
+        let rel = SUBTYPING e in
+        with_context "check_subtype" (Some (CtxRel t0 rel t1))
+          (fun _ -> check_relation g rel t0 t1)
+          ctx)
+      None
+      "FStar.TypeChecker.Core.check_subtype"
 
 and memo_check (g:env) (e:term)
   : result (effect_label & typ)
@@ -1990,10 +2010,24 @@ let check_term_top_gh g e topt (must_tot:bool) (gh:option guard_handler_t)
     in
     if FStar.Options.profile_enabled None "FStar.TypeChecker.Core.check_term_top"
     then (
-      let cs = report_cache_stats() in
-      BU.print2 "Cache_stats { hits = %s; misses = %s }\n"
-                     (BU.string_of_int cs.hits)
-                     (BU.string_of_int cs.misses)
+      FStar.Hash.max_bucket_stats table
+        (fun hash_opt entries ->
+          match hash_opt with
+          | None -> ()
+          | Some h ->
+            BU.print2 "Hash %s had the largest bucket with size %s and entries {{\n"
+                      (string_of_int h)
+                      (string_of_int (List.length entries));
+            List.iteri (fun i (t, _) -> BU.print3 "%s (hash code %s): %s\n" 
+                                               (BU.string_of_int i)
+                                               (FStar.Hash.string_of_hash_code (FStar.Syntax.Hash.ext_hash_term_no_memo t))
+                                               (P.term_to_string t))
+                       entries;
+            BU.print_string "}}\n")
+      // let cs = report_cache_stats() in
+      // BU.print2 "Cache_stats { hits = %s; misses = %s }\n"
+      //                (BU.string_of_int cs.hits)
+      //                (BU.string_of_int cs.misses)
     );
     res
     )
